src/StateMonad.v
@@ -1,33 +1,6 @@
 Require Import Coq.Logic.FunctionalExtensionality.
+Require Export compiler.Monad.
 
-Class Monad(M: Type -> Type) := mkMonad {
-  Bind: forall {A B}, M A -> (A -> M B) -> M B;
-  Return: forall {A}, A -> M A;
-
-  left_identity: forall {A B} (a: A) (f: A -> M B),
-    Bind (Return a) f = f a;
-  right_identity: forall {A} (m: M A),
-    Bind m Return = m;
-  associativity: forall {A B C} (m: M A) (f: A -> M B) (g: B -> M C),
-    Bind (Bind m f) g = Bind m (fun x => Bind (f x) g)
-}.
-
-Notation "x <- m1 ; m2" := (Bind m1 (fun x => m2))
-  (right associativity, at level 60).
-Notation "m1 ;; m2" := (Bind m1 (fun _ => m2))
-  (right associativity, at level 60).
-
-Instance option_Monad: Monad option := {|
-  Bind := fun {A B: Type} (o: option A) (f: A -> option B) => match o with
-          | Some x => f x
-          | None => None
-          end;
-  Return := fun {A: Type} (a: A) => Some a
-|}.
-- intros. reflexivity.
-- intros. destruct m; reflexivity.
-- intros. destruct m; reflexivity.
-Defined.
 
 Definition State(S A: Type) := S -> (A * S).
 
