src/Common.v
@@ -1,0 +1,21 @@
+Require Export compiler.Monad.
+Require Export compiler.Decidable.
+Require Export bbv.Word.
+
+Class Map(T K V: Type) := mMap {
+  empty: T;
+  get: T -> K -> option V;
+  put: T -> K -> V -> T;
+  (* TODO probably needs some properties *)
+}.
+
+Instance Function_Map(K V: Type){decK: DecidableEq K}: Map (K -> option V) K V := {|
+  empty := fun _ => None;
+  get := id;
+  put := fun (m: K -> option V) (k: K) (v: V) =>
+           fun (k': K) => if dec (k = k') then Some v else m k'
+|}.
+
+Global Instance dec_eq_word : forall sz, DecidableEq (word sz) := weq.
+
+Inductive binop: Set := OPlus | OMinus | OTimes.
