src/Monad.v
@@ -1,0 +1,31 @@
+Require Import Coq.Logic.FunctionalExtensionality.
+
+Class Monad(M: Type -> Type) := mkMonad {
+  Bind: forall {A B}, M A -> (A -> M B) -> M B;
+  Return: forall {A}, A -> M A;
+
+  left_identity: forall {A B} (a: A) (f: A -> M B),
+    Bind (Return a) f = f a;
+  right_identity: forall {A} (m: M A),
+    Bind m Return = m;
+  associativity: forall {A B C} (m: M A) (f: A -> M B) (g: B -> M C),
+    Bind (Bind m f) g = Bind m (fun x => Bind (f x) g)
+}.
+
+Notation "x <- m1 ; m2" := (Bind m1 (fun x => m2))
+  (right associativity, at level 60).
+Notation "m1 ;; m2" := (Bind m1 (fun _ => m2))
+  (right associativity, at level 60).
+
+Instance option_Monad: Monad option := {|
+  Bind := fun {A B: Type} (o: option A) (f: A -> option B) => match o with
+          | Some x => f x
+          | None => None
+          end;
+  Return := fun {A: Type} (a: A) => Some a
+|}.
+- intros. reflexivity.
+- intros. destruct m; reflexivity.
+- intros. destruct m; reflexivity.
+Defined.
+
