src/ResMonad.v
@@ -1,0 +1,30 @@
+Require Import compiler.Monad.
+Require Import compiler.Tactics.
+
+Inductive Res(A: Type): Type :=
+| Success(a: A): Res A
+| Fail: Res A
+| OutOfFuel: Res A.
+
+Arguments Success {A}.
+Arguments Fail {A}.
+Arguments OutOfFuel {A}.
+
+Instance Res_Monad: Monad Res := {| 
+  Bind := fun {A B: Type} (r: Res A) (f: A -> Res B) => match r with
+          | Success a => f a
+          | Fail => Fail
+          | OutOfFuel => OutOfFuel
+          end;
+  Return := fun {A: Type} (a: A) => Success a
+|}.
+- intros; reflexivity.
+- intros; destruct_one_match; reflexivity.
+- intros; repeat destruct_one_match; reflexivity.
+Defined.
+
+Definition option2res{A: Type}(o: option A): Res A :=
+  match o with
+  | Some a => Success a
+  | None => Fail
+  end.
