src/Tactics.v
@@ -1,0 +1,9 @@
+
+Ltac destruct_one_match :=
+  match goal with
+  | [ |- context[match ?e with _ => _ end] ] =>
+      is_var e; destruct e
+  | [ |- context[match ?e with _ => _ end] ] =>
+      let E := fresh "E" in destruct e eqn: E
+  end.
+
